AssocArray refactor

Algorithm/Data/Classes/AssocArray.lean
@@ -7,94 +7,99 @@ import Mathlib.Data.Fintype.Basic
 import Mathlib.Data.Setoid.Basic
 import Std.Data.Array.Lemmas
 
-/-- `AssocArray ι α M` is a data structure that acts like a finitely supported function `ι → α`
+/-- `AssocArray A ι α` is a data structure that acts like a finitely supported function `ι → α`
   with single point update operation. -/
-class AssocArray (ι : outParam <| Type _) [DecidableEq ι]
-    (α : outParam <| Type _) [Inhabited α] (M : Type _) where
-  empty : M
-  set : M → ι → α → M
-  get : M → ι → α
-  get_set : get (set a i v) = Function.update (get a) i v
+class AssocArray (A : Type*) (ι : outParam Type*) [DecidableEq ι]
+    (α : outParam Type*) [Inhabited α] where
+  empty : A
+  update : A → ι → α → A
+  get : A → ι → α
+  get_update {a i v} : get (update a i v) = Function.update (get a) i v
   get_empty : get empty = Function.const _ default
 
-attribute [simp] AssocArray.get_set AssocArray.get_empty
+attribute [simp] AssocArray.get_update AssocArray.get_empty
+
+instance {A ι : Type*} [DecidableEq ι] {α : Type*} [Inhabited α] [AssocArray A ι α] :
+    GetElem A ι α fun _ _ ↦ True where
+  getElem a i _ := AssocArray.get a i
 
 namespace Array
+variable {α : Type*} {n : ℕ}
 
 lemma get_fin_set (a : Array α) (i : Fin a.size) (v : α) (j : Fin (set a i v).size) :
     (a.set i v).get j = if i.1 = j.1 then v else a[j.1] := by
   rw [get_eq_getElem, get_set]
 
-instance [Inhabited α] : AssocArray (Fin n) α {a : Array α // a.size = n} where
+instance [Inhabited α] : AssocArray {a : Array α // a.size = n} (Fin n) α where
   empty := ⟨.mk <| List.replicate n default, List.length_replicate _ _⟩
-  set a i v := ⟨a.1.set (Fin.cast a.2.symm i) v, (Array.size_set _ _ _).trans a.2⟩
+  update a i v := ⟨a.1.set (Fin.cast a.2.symm i) v, (Array.size_set _ _ _).trans a.2⟩
   get a i := a.1.get (Fin.cast a.2.symm i)
-  get_set {a i v} := by
-    simp_rw [get_fin_set]; simp [Function.update, Fin.val_eq_val, eq_comm (a := i)]
+  get_update {a i v} := by
+    simp_rw [get_fin_set]
+    simp [Function.update, Fin.val_eq_val, eq_comm (a := i)]
   get_empty := by
-    ext; simp [get]
+    ext
+    simp [get]
 
 end Array
 
 namespace AssocArray
 
-class Ext (ι : outParam <| Type _) [DecidableEq ι]
-    (α : outParam <| Type _) [Inhabited α] (M : Type _) [AssocArray ι α M] where
-  ext : ∀ {m₁ m₂ : M}, get m₁ = get m₂ → m₁ = m₂
+class Ext (A : Type*) (ι : outParam Type*) [DecidableEq ι]
+    (α : outParam Type*) [Inhabited α] [AssocArray A ι α] where
+  ext : ∀ {m₁ m₂ : A}, get m₁ = get m₂ → m₁ = m₂
 
-variable {ι : Type _} [DecidableEq ι] {α : Type _} [Inhabited α] {M : Type _} [AssocArray ι α M]
+variable {A ι : Type*} [DecidableEq ι] {α : Type*} [Inhabited α] [AssocArray A ι α]
 
-variable (M)
+variable (A)
 
-def Quotient := @_root_.Quotient M (Setoid.ker get)
+def Quotient := @_root_.Quotient A (Setoid.ker get)
 
-instance : AssocArray ι α (Quotient M) where
+instance : AssocArray (Quotient A) ι α where
   empty := ⟦empty⟧
-  set q i v := q.map' (set · i v) (fun _ _ hm ↦ (Eq.congr get_set get_set).mpr (by rw [hm]))
+  update q i v := q.map' (update · i v) (fun _ _ hm ↦ (Eq.congr get_update get_update).mpr (by rw [hm]))
   get := Quotient.lift get (fun _ _ ↦ id)
-  get_set {q i v} := q.inductionOn (fun _ ↦ get_set)
+  get_update {q i v} := q.inductionOn (fun _ ↦ get_update)
   get_empty := get_empty
 
-instance : Ext ι α (Quotient M) where
+instance : Ext (Quotient A) ι α where
   ext {m₁ m₂} := m₂.inductionOn <| m₁.inductionOn (fun _ _ ha ↦ Quotient.sound ha)
 export Ext (ext)
 
-def listIndicator (l : List ι) (f : ∀ i ∈ l, α) : M :=
+def listIndicator (l : List ι) (f : ∀ i ∈ l, α) : A :=
   match l with
   | [] => empty
-  | (i :: l) => set (listIndicator l (fun i hi ↦ f i (List.mem_cons_of_mem _ hi)))
+  | (i :: l) => update (listIndicator l (fun i hi ↦ f i (List.mem_cons_of_mem _ hi)))
     i (f i (List.mem_cons_self _ _))
 
-variable {M}
+variable {A}
 
 lemma get_listIndicator (l : List ι) (f : ∀ i ∈ l, α) :
-    get (listIndicator M l f) = (fun i ↦ if hi : i ∈ l then f i hi else default) :=
+    get (listIndicator A l f) = (fun i ↦ if hi : i ∈ l then f i hi else default) :=
   match l with
   | [] => by simp [listIndicator, get_empty, Function.const]
   | (i :: l) => by
     ext j
-    rw [listIndicator, get_set, Function.update_apply]
-    split_ifs with h₁ h₂
+    rw [listIndicator, get_update, Function.update_apply]
+    split_ifs with h₁ h₂ h₂
     · simp [h₁]
     · simp [h₁] at h₂
-    · rename_i h₂ -- a `split_ifs` bug
-      simp_rw [get_listIndicator, dif_pos (List.mem_of_ne_of_mem h₁ h₂)]
-    · rename_i h₂ -- a `split_ifs` bug
-      simp_rw [get_listIndicator, dif_neg (List.not_mem_of_not_mem_cons h₂)]
+    · simp_rw [get_listIndicator, dif_pos (List.mem_of_ne_of_mem h₁ h₂)]
+    · simp_rw [get_listIndicator, dif_neg (List.not_mem_of_not_mem_cons h₂)]
 
-variable [Ext ι α M]
-variable (M)
+variable [Ext A ι α]
+variable (A)
 
-def indicator (s : Finset ι) (f : ∀ i ∈ s, α) : M :=
+def indicator (s : Finset ι) (f : ∀ i ∈ s, α) : A :=
   let this := Equiv.subtypeQuotientEquivQuotientSubtype (fun l : List ι ↦ ↑l = s.1)
     (fun m ↦ m = s.1) (fun i ↦ Iff.rfl) (fun _ _ ↦ Iff.rfl) ⟨s.1, rfl⟩
-  this.liftOn (fun l ↦ listIndicator M l (fun i hi ↦ f i (l.2 ▸ hi : i ∈ s.1)))
+  this.liftOn (fun l ↦ listIndicator A l (fun i hi ↦ f i (l.2 ▸ hi : i ∈ s.1)))
     (fun l₁ l₂ hl ↦ ext <| by simp_rw [get_listIndicator, List.Perm.mem_iff hl])
 
-variable {M}
+variable {A}
 
 lemma get_indicator (s : Finset ι) (f : ∀ i ∈ s, α) :
-    get (indicator M s f) = (fun i ↦ if hi : i ∈ s then f i hi else default) := by
+    get (indicator A s f) = (fun i ↦ if hi : i ∈ s then f i hi else default) := by
   unfold indicator
   change _ = (fun i ↦ if hi : i ∈ s.1 then _ else _)
   obtain ⟨l, hl⟩ := s.1.exists_rep
@@ -104,14 +109,14 @@ lemma get_indicator (s : Finset ι) (f : ∀ i ∈ s, α) :
   rw [get_listIndicator]
   rfl
 
-variable (M)
+variable (A)
 
-def ofFun [Fintype ι] (f : ι → α) : M := indicator M Finset.univ (fun i _ ↦ f i)
+def ofFun [Fintype ι] (f : ι → α) : A := indicator A Finset.univ (fun i _ ↦ f i)
 
-variable {M}
+variable {A}
 
 lemma get_ofFun [Fintype ι] (f : ι → α) :
-    get (ofFun M f) = f :=
+    get (ofFun A f) = f :=
   (get_indicator _ _).trans <| funext fun _ ↦ dif_pos <| Finset.mem_univ _
 
 end AssocArray
