lakefile.lean
@@ -1,11 +1,14 @@
 import Lake
 open Lake DSL
 
-package algorithm
+package algorithm {
+  moreServerArgs := #["-DautoImplicit=false"]
+}
 
 require mathlib from git "https://github.com/leanprover-community/mathlib4.git" @ "master"
 
 @[default_target]
 lean_lib Algorithm {
   roots := #[`Algorithm]
+  moreLeanArgs := #["-DautoImplicit=false"]
 }
